src/Assembly/Pseudize.v
@@ -1,0 +1,44 @@
+Require Export Bedrock.Word Bedrock.Nomega.
+Require Import NArith List.
+Require Import Pseudo State Wordize.
+
+Module Conversion.
+  Import Pseudo ListNotations StateCommon.
+
+  Definition run {n m w s} (prog: @Pseudo w s n m) (inList: list (word w)) : list (word w) :=  
+    match (pseudoEval prog (inList, TripleM.empty N, None)) with
+    | Some (outList, _, _) => outList
+    | _ => []
+    end.
+
+  Lemma pseudo_plus: forall {w s n} (p0 p1: @Pseudo w s n 1) x out0 out1 b,
+      (b <= Npow2 w)%N
+    -> ((&out0)%w < b)%N
+    -> ((&out1)%w < (Npow2 w - b))%N
+    -> run p0 x = [out0]
+    -> run p1 x = [out1]
+    -> run (p0 :+: p1)%p x = [out0 ^+ out1].
+  Proof.
+    intros; unfold run in *; simpl.
+    destruct (pseudoEval p0 _) as [r0|], (pseudoEval p1 _) as [r1|].
+    destruct r0 as [r0 rc0], r1 as [r1 rc1].
+    destruct r0 as [r0 rm0], r1 as [r1 rm1].
+
+    - subst; simpl.
+      destruct ((& out0)%w + (& out1)%w ?= Npow2 w)%N; simpl;
+        rewrite (wordize_plus out0 out1 b); try assumption;
+        rewrite NToWord_wordToN; intuition.
+
+    - inversion H3.
+
+    - inversion H2.
+
+    - inversion H2.
+  Qed.
+
+  Program Definition ex0: Program Unary32 := ($0 :-: $0)%p.
+
+  Eval vm_compute in (run ex0 [natToWord _ 7]).
+
+End Conversion.
+
